src/Distributions/BernoulliExpNeg/Equivalence.dfy
@@ -18,7 +18,7 @@ module BernoulliExpNeg.Equivalence {
   opaque ghost predicate CaseLe1LoopInvariant(gamma: Rationals.Rational, oldS: Rand.Bitstream, a: bool, k: nat, s: Rand.Bitstream)
     requires 0 <= gamma.numer <= gamma.denom
   {
-    Model.GammaLe1Loop(gamma)((true, 0))(oldS) == Model.GammaLe1Loop(gamma)((a, k))(s)
+    Model.Le1Loop(gamma)((true, 0))(oldS) == Model.Le1Loop(gamma)((a, k))(s)
   }
 
   /*******
@@ -29,25 +29,25 @@ module BernoulliExpNeg.Equivalence {
     requires gamma.numer > 0
     requires prevGamma.denom == gamma.denom
     requires prevGamma.numer == gamma.numer + gamma.denom
-    requires Model.SampleGammaLe1(Rationals.Int(1))(prevS) == Monad.Result(b, s)
+    requires Model.SampleLe1(Rationals.Int(1))(prevS) == Monad.Result(b, s)
     ensures Model.Sample(prevGamma)(prevS) == if b then Model.Sample(gamma)(s) else Monad.Result(false, s)
   {
     reveal Model.Sample();
   }
 
-  lemma GammaLe1LoopUnroll(gamma: Rationals.Rational, ak: (bool, nat), s: Rand.Bitstream)
+  lemma Le1LoopUnroll(gamma: Rationals.Rational, ak: (bool, nat), s: Rand.Bitstream)
     requires 0 <= gamma.numer <= gamma.denom
     requires ak.0
-    ensures Model.GammaLe1Loop(gamma)(ak)(s) == Monad.Bind(Model.GammaLe1LoopIter(gamma)(ak), Model.GammaLe1Loop(gamma))(s)
+    ensures Model.Le1Loop(gamma)(ak)(s) == Monad.Bind(Model.Le1LoopIter(gamma)(ak), Model.Le1Loop(gamma))(s)
   {
-    Model.GammaLe1LoopTerminatesAlmostSurely(gamma);
+    Model.Le1LoopTerminatesAlmostSurely(gamma);
     calc {
-      Model.GammaLe1Loop(gamma)(ak)(s);
-      { reveal Model.GammaLe1Loop(); }
-      Loops.While(Model.GammaLe1LoopCondition, Model.GammaLe1LoopIter(gamma))(ak)(s);
-      { reveal Model.GammaLe1Loop();
-        Loops.WhileUnroll(Model.GammaLe1LoopCondition, Model.GammaLe1LoopIter(gamma), ak, s); }
-      Monad.Bind(Model.GammaLe1LoopIter(gamma)(ak), Model.GammaLe1Loop(gamma))(s);
+      Model.Le1Loop(gamma)(ak)(s);
+      { reveal Model.Le1Loop(); }
+      Loops.While(Model.Le1LoopCondition, Model.Le1LoopIter(gamma))(ak)(s);
+      { reveal Model.Le1Loop();
+        Loops.WhileUnroll(Model.Le1LoopCondition, Model.Le1LoopIter(gamma), ak, s); }
+      Monad.Bind(Model.Le1LoopIter(gamma)(ak), Model.Le1Loop(gamma))(s);
     }
   }
 
@@ -65,15 +65,15 @@ module BernoulliExpNeg.Equivalence {
     requires bernoulli: Monad.Result(a' , s') == Bernoulli.Model.Sample(gamma.numer, k' * gamma.denom)(s)
     ensures CaseLe1LoopInvariant(gamma, oldS, a', k', s')
   {
-    assert iter: Monad.Result((a', k'), s') == Model.GammaLe1LoopIter(gamma)((true, k))(s) by {
+    assert iter: Monad.Result((a', k'), s') == Model.Le1LoopIter(gamma)((true, k))(s) by {
       reveal bernoulli;
     }
     calc {
-      Model.GammaLe1Loop(gamma)((true, 0))(oldS);
+      Model.Le1Loop(gamma)((true, 0))(oldS);
       { reveal CaseLe1LoopInvariant(); reveal inv; }
-      Model.GammaLe1Loop(gamma)((true, k))(s);
-      { reveal iter; GammaLe1LoopUnroll(gamma, (true, k), s); }
-      Model.GammaLe1Loop(gamma)((a', k'))(s');
+      Model.Le1Loop(gamma)((true, k))(s);
+      { reveal iter; Le1LoopUnroll(gamma, (true, k), s); }
+      Model.Le1Loop(gamma)((a', k'))(s');
     }
     reveal CaseLe1LoopInvariant();
   }
@@ -82,13 +82,13 @@ module BernoulliExpNeg.Equivalence {
     requires 0 <= gamma.numer <= gamma.denom
     requires CaseLe1LoopInvariant(gamma, oldS, false, k, s)
     requires c <==> (k % 2 == 1)
-    ensures Monad.Result(c, s) == Model.SampleGammaLe1(gamma)(oldS)
+    ensures Monad.Result(c, s) == Model.SampleLe1(gamma)(oldS)
   {
     calc {
-      Model.GammaLe1Loop(gamma)((true, 0))(oldS);
+      Model.Le1Loop(gamma)((true, 0))(oldS);
       { reveal CaseLe1LoopInvariant(); }
-      Model.GammaLe1Loop(gamma)((false, k))(s);
-      { reveal Model.GammaLe1Loop(); }
+      Model.Le1Loop(gamma)((false, k))(s);
+      { reveal Model.Le1Loop(); }
       Monad.Result((false, k), s);
     }
   }
